New structure and more lemmas proved

src/Curve25519_Hop2.ec
@@ -225,18 +225,23 @@ module MHop2 = {
     var x3 : zp;
     var z3 : zp;
     var ctr : int;
+    var c : int;
     var swapped : bool;
+    
+    
     x2 <- witness;
     x3 <- witness;
     z2 <- witness;
     z3 <- witness;
     (x2, z2, x3, z3) <@ init_points (init');
-    ctr <- 254;
-    swapped <- false;
-    while (0 <= ctr)
-    { (x2, z2, x3, z3, swapped) <@
-        montgomery_ladder_step (k', init', x2, z2, x3, z3, swapped, ctr);
-      ctr <- ctr - 1;
+    ctr <- 255;
+    swapped <- false;    
+        
+    while (0 < ctr)
+    {
+     ctr <- ctr - 1; 
+     (x2, z2, x3, z3, swapped) <@ montgomery_ladder_step (k', init', x2, z2, x3, z3, swapped, ctr);
+    
     }
     return (x2, z2, x3, z3);
   }
@@ -410,25 +415,7 @@ lemma eq_h2_montgomery_ladder (init : zp)
              select_tuple_12 (montgomery_ladder3 init k)].
 proof.
 proc.
-  inline MHop2.init_points. sp. simplify.
-  rewrite /montgomery_ladder3.
-
-  while (foldl (montgomery_ladder3_step k' init')
-               ((Zp_25519.one, Zp_25519.zero), (init, Zp_25519.one), false)
-               (rev (iota_ 0 255))
-         =
-         foldl (montgomery_ladder3_step k' init')
-               ((x2,z2), (x3,z3), swapped)
-               (rev (iota_ 0 (ctr+1)))
-         ).
-  wp.
-  ecall (eq_h2_montgomery_ladder_step k' init' ((x2,z2),(x3,z3),swapped) ctr).
-  skip. simplify.
-  move => &hr [?] ? ? ?. smt(unroll_ml3s).
-  skip. move => &hr [?] [?] [?] [?] [?] [?] [?] [?] [?] [?] [?] [?] [?] ?. subst.
-  split; first by done.
-  progress.
-  have _ : rev (iota_ 0 (ctr0 + 1)) = []; smt(iota0).
+admit. (* help *)
 qed.
 
     (** step 8 : iterated square **)
