src/Curve25519_Hop4.ec
@@ -1,235 +1,18 @@
 require import AllCore Bool List Int IntDiv StdOrder CoreMap Real Zp_25519 Ring EClib Distr.
-from Jasmin require import JModel JWord_array.
 require import Curve25519_Spec.
 require import Curve25519_Hop1.
 require import Curve25519_Hop2.
 require import Curve25519_Hop3.
 require import Curve25519_ref4.
-import Zp_25519 ZModpRing.
-import Curve25519_Spec Curve25519_Hop1 Curve25519_Hop2 Curve25519_ref4 Array4 Array32 StdOrder.IntOrder.
-require import W64limbs.
+require import Curve25519_auto.
+import Zp_25519.
+import Curve25519_Spec Curve25519_auto Curve25519_Hop1 Curve25519_Hop2 Curve25519_ref4 Array4 Array32 StdOrder.IntOrder.
 
 
-
-(** representation : move to another file/use rep3/5 **)
-type Rep4 = W64.t Array4.t.
-type Rep32 = W8.t Array32.t.
-
-
-op valRep4  (x : Rep4) : int = val_limbs64 (Array4.to_list x).
-op valRep4List  (x : W64.t list) : int = val_limbs64(x).
-op inzpRep4 (x : Rep4) : zp  = inzp (valRep4 x) axiomatized by inzpRep4E.
-op inzpRep4List (x: W64.t list) : zp = inzp (valRep4List x) axiomatized by inzpRep4ListE.
-
-abbrev zpcgrRep4 (x : Rep4) (z : int) : bool = zpcgr (valRep4 x) z.
-
-op valRep32  (x : Rep32) : int = val_limbs8 (Array32.to_list x).
-op inzpRep32 (x : Rep32) : zp  = inzp (valRep32 x) axiomatized by inzpRep32E.
-(** ************************************* **)
-
-(** step 0 : add sub mul sqr - all done by auto **)
-
-equiv eq_h4_add : MHop2.add ~ M.__add4_rrs:
-   f{1} = inzpRep4 f{2} /\
-   g{1} = inzpRep4 g{2}
-    ==>
-   res{1} = inzpRep4 res{2}.
-proof. 
- proc.  
- admit.
-qed.
-
-equiv eq_h4_sub : MHop2.sub ~ M.__sub4_rrs:
-   f{1} = inzpRep4 f{2} /\
-   g{1} = inzpRep4 gs{2}
-    ==>
-   res{1} = inzpRep4 res{2}.
-proof.
-proc.
-admit.
-qed.
-
-equiv eq_h4_mul_a24 : MHop2.mul_a24 ~ M.__mul4_a24_rs:
-   f{1} = inzpRep4 xa{2} /\
-   a24{1} = to_uint a24{2}
-    ==>
-   res{1} = inzpRep4 res{2}.
-proof.
-  proc.
- admit.
-qed.
-
-equiv eq_h4_mul_rss : MHop2.mul ~ M.__mul4_rss:
-   f{1} = inzpRep4 xa{2} /\
-   g{1} = inzpRep4 ya{2}
-    ==>
-   res{1} = inzpRep4 res{2}.
-proof.
-proc.
-admit.
-qed.
-
-equiv eq_h4_sqr : MHop2.sqr ~ M.__sqr4_rs:
-    f{1} = inzpRep4 xa{2}
-    ==>
-    res{1} = inzpRep4 res{2}.
-proof.
-admit.
-qed.
-
-(** step 0.5 : transitivity stuff **)
-equiv eq_h4_add_ssr : MHop2.add ~ M.__add4_ssr:
-   f{1} = inzpRep4 fs{2} /\
-   g{1} = inzpRep4 g{2}
-    ==>
-   res{1} = inzpRep4 res{2}.
-proof.
-proc.
-admit.
-qed.
-
-
-equiv eq_h4_add_sss : MHop2.add ~ M.__add4_sss:
-   f{1} = inzpRep4 fs{2} /\
-   g{1} = inzpRep4 gs{2}
-    ==>
-   res{1} = inzpRep4 res{2}.
-proof.
-proc.
-admit.
-qed.
-
-equiv eq_h4_add_rrs : MHop2.add ~ M.__add4_rrs:
-   f{1} = inzpRep4 f{2} /\
-   g{1} = inzpRep4 g{2}
-    ==>
-   res{1} = inzpRep4 res{2}.
-proof.
-proc.
-admit.
-qed.
-
-
-equiv eq_h4_sub_ssr : MHop2.sub ~ M.__sub4_ssr:
-   f{1} = inzpRep4 fs{2} /\
-   g{1} = inzpRep4 g{2}
-    ==>
-   res{1} = inzpRep4 res{2}.
-proof.
-proc.
-admit.
-qed.
-
-equiv eq_h4_sub_rsr : MHop2.sub ~ M.__sub4_rsr:
-   f{1} = inzpRep4 fs{2} /\
-   g{1} = inzpRep4 g{2}
-    ==>
-   res{1} = inzpRep4 res{2}.
-proof.
-proc.
-admit.
-qed.
-
-equiv eq_h4_sub_sss : MHop2.sub ~ M.__sub4_sss:
-   f{1} = inzpRep4 fs{2} /\
-   g{1} = inzpRep4 gs{2}
-    ==>
-   res{1} = inzpRep4 res{2}.
-proof.
-proc.
-admit.
-qed.
-
-equiv eq_h4_mul_a24_ss : MHop2.mul_a24 ~ M.__mul4_a24_ss:
-   f{1} = inzpRep4 xa{2} /\
-   a24{1} = to_uint a24{2}
-    ==>
-   res{1} = inzpRep4 res{2}.
-proof.
-proc.
-admit.
-qed.
-
-equiv eq_h4_mul_sss : MHop2.mul ~ M.__mul4_sss:
-   f{1} = inzpRep4 xa{2} /\
-   g{1} = inzpRep4 ya{2}
-    ==>
-   res{1} = inzpRep4 res{2}.
-proof.
-proc.
-admit.
-qed.
-
-equiv eq_h4_mul_pp : MHop2.mul ~ M._mul4_pp:
-   f{1} = inzpRep4 xa{2} /\
-   g{1} = inzpRep4 ya{2}
-    ==>
-   res{1} = inzpRep4 res{2}.
-proof.
-proc.
-admit.
-qed.
-
-
-equiv eq_h4_mul_ss : MHop2.mul ~ M._mul4_ss_:
-   f{1} = inzpRep4 xa{2} /\
-   g{1} = inzpRep4 ya{2}
-    ==>
-   res{1} = inzpRep4 res{2}.
-proof.
-proc.
-admit.
-qed.
-
-
-equiv eq_h4_sqr_rs : MHop2.sqr ~ M.__sqr4_rs:
-    f{1} = inzpRep4 xa{2}
-    ==>
-    res{1} = inzpRep4 res{2}.
-proof.
-proc.
-admit.
-qed.
-
-equiv eq_h4_sqr_ss : MHop2.sqr ~ M._sqr4_ss_:
-    f{1} = inzpRep4 xa{2}
-    ==>
-    res{1} = inzpRep4 res{2}.
-proof.
-proc.
-admit.
-qed.
-
-equiv eq_h4_sqr_ss_ : MHop2.sqr ~ M.__sqr4_ss:
-    f{1} = inzpRep4 xa{2}
-    ==>
-    res{1} = inzpRep4 res{2}.
-proof.
-proc.
-admit.
-qed.
-
-equiv eq_h4_sqr_s_ : MHop2.sqr ~ M._sqr4_s_:
-    f{1} = inzpRep4 x{2}
-    ==>
-    res{1} = inzpRep4 res{2}.
-proof.
-proc.
-admit.
-qed.
-
-equiv eq_h4_sqr_p : MHop2.sqr ~ M._sqr4_p:
-    f{1} = inzpRep4 xa{2}
-    ==>
-    res{1} = inzpRep4 res{2}.
-proof.
-proc.
-admit.
-qed.
 
 (** init **)
 
-equiv eq_init_points4 :
+equiv eq_h4_init_points :
     MHop2.init_points ~ M.__init_points4 : 
 init{1} = inzpRep4 initr{2}
 ==> 
@@ -247,42 +30,12 @@ rewrite /valRep4 /to_list /mkseq -iotaredE  => />.
 rewrite /H6  /H0 /H3 /H2 /Zp_25519.zero /set0_64_ /inzpRep4 // /valRep4 /to_list /mkseq -iotaredE  => />.
 qed. 
 
-(** step 1 : decode_scalar_25519 **)
- equiv eq_h4_decode_scalar_25519 :
-  MHop2.decode_scalar ~ M.__decode_scalar:
-  inzp(W256.to_uint(k'{1})) = inzpRep4 k{2}
-  ==> 
-   inzp(W256.to_uint res{1}) = inzpRep32  res{2}. 
-proof.
-admit. (* AUTO *)
-qed.
-
-
-(** step 2 : decode_u_coordinate **)
-equiv eq_h4_decode_u_coordinate :
-  MHop2.decode_u_coordinate ~ M.__decode_u_coordinate4:
-  inzp(W256.to_uint(u'{1})) = inzpRep4 u{2}
-  ==> 
-  res{1} = inzpRep4 res{2}.
-proof.
-admit. (* AUTO MSB already 0 -  ask tiago *)
-qed.
-
 equiv eq_h4_decode_u_coordinate_base :
   MHop2.decode_u_coordinate_base ~ M.__decode_u_coordinate_base4:
   true ==> res{1} = inzpRep4 res{2}.
 proof.
 proc. wp. skip. move => &1 &2 H.
 rewrite /inzpRep4. congr. rewrite /valRep4 /to_list /mkseq -iotaredE => />.
-qed.
-
-(** step 3 : ith_bit **)
-equiv eq_h4_ith_bit :
-  MHop2.ith_bit ~ M.__ith_bit :
-  inzp (W256.to_uint k'{1}) = inzpRep32 k{2} /\  (ctr{1} = to_uint ctr{2}) ==> b2i res{1} = to_uint res{2}.
-proof.
-proc.
-admit. (* AUTO *)
 qed.
 
 
@@ -377,18 +130,18 @@ equiv eq_h4_montgomery_ladder_step :
    res{1}.`4 = inzpRep4 res{2}.`4 /\
    b2i res{1}.`5 = to_uint res{2}.`5.
 proof.
-proc => /=. 
-call eq_h4_add_and_double. wp.
-call eq_h4_cswap. wp.
-call eq_h4_ith_bit. skip. 
-move => &1 &2 [H0] [H1] [H2] [H3] [H4] [H5] [H6] H7. split.   
-auto => />. rewrite H0. 
-move => [H8 H9] H10 H11 H12 H13 H14. 
-split;  auto => />. rewrite /H14 /H13. 
-rewrite /b2i. 
-case: (swapped{1} ^^ H10).
-move => *. smt(@W64). 
-move => *. smt(@W64). 
+    proc => /=. 
+    call eq_h4_add_and_double. wp.
+    call eq_h4_cswap. wp.
+    call eq_h4_ith_bit. skip. 
+    move => &1 &2 [H0] [H1] [H2] [H3] [H4] [H5] [H6] H7. split.   
+    auto => />. rewrite H0. 
+    move => [H8 H9] H10 H11 H12 H13 H14. 
+    split;  auto => />. rewrite /H14 /H13. 
+    rewrite /b2i. 
+    case: (swapped{1} ^^ H10).
+    move => *. smt(@W64). 
+    move => *. smt(@W64). 
 qed.   
 
 (** step 7 : montgomery_ladder **)
@@ -400,10 +153,25 @@ equiv eq_h4_montgomery_ladder :
    res{1}.`1 = inzpRep4 res{2}.`1 /\
    res{1}.`2 =inzpRep4  res{2}.`2.
 proof.
-proc. sp. wp. swap 1 2. sp. 
-while(-1 <= ctr{1} /\ -1 <= to_uint ctr{2} /\ x2{1} = inzpRep4 x2{2} /\ z2{1} = inzpRep4 z2r{2}).
-wp. sp. admit. admit.
-
+    proc. wp. sp. 
+    unroll {1} 4. 
+    rcondt {1} 4. progress. inline MHop2.init_points.
+    wp. sp. skip. progress.
+    while(
+          inzp (to_uint k'{1}) = inzpRep32 k{2}             /\ 
+          ctr{1} = to_uint ctr{2}                          /\ 
+          inzp (to_uint k'{1}) = inzpRep32 k{2}            /\
+          init'{1} = inzpRep4 us{2}                        /\ 
+          x2{1} = inzpRep4 x2{2}                           /\
+          x3{1} = inzpRep4 x3{2}                           /\
+          z2{1} = inzpRep4 z2r{2}                          /\
+          z3{1} = inzpRep4 z3{2}                           /\
+          b2i swapped{1} = to_uint swapped{2}).
+    wp. sp. call eq_h4_montgomery_ladder_step. skip. progress.
+    rewrite to_uintB. rewrite uleE to_uint1 => />. smt(). rewrite to_uint1 => />.
+    rewrite ultE to_uintB. rewrite uleE to_uint1. smt().
+    rewrite to_uint1 to_uint0. trivial. smt(@W64).  
+    call eq_h4_montgomery_ladder_step. wp. call eq_h4_init_points. skip. done.
 qed.
 
  (** step 8 : iterated square, may be error in variable names, ened to chec  **)
@@ -495,16 +263,6 @@ proof.
 qed.
 
 
-(** step 10 : encode point **)
-equiv eq_h4_encode_point : 
-  MHop2.encode_point ~ M.__encode_point4:
-  x2{1} = inzpRep4 x2{2} /\ 
-  z2{1} = inzpRep4 z2r{2}
-  ==>
-  inzp (to_uint res{1}) =  inzpRep4 res{2}.
-proof.
-admit. (* AUTO *)
-qed.
 
 (** step 11 : scalarmult **)
 
@@ -533,17 +291,14 @@ call eq_h4_decode_scalar_25519.
 wp. skip. progress.
 qed.
 
-(*
+
 equiv eq_h4_scalarmult_ptr : (* how to get address *)
   MHop2.scalarmult ~ M.__curve25519_ref4_ptr:
-  inzp(W256.to_uint k'{1}) = inzpRep4 kp{2} /\  inzp (to_uint u'{1}) = inzpRep4 up{2}
-  ==>
-  inzp(W256.to_uint res{1}) = inzpRep4 res{2}. 
-proof.
+  true ==> true.
 proof.
 admit.
 qed.
-*)
+
 
 equiv eq_h4_scalarmult_base :
   MHop2.scalarmult_base ~ M._curve25519_ref4_base:
