src/Curve25519_auto.ec
@@ -1,0 +1,266 @@
+require import Int Bool Zp_25519 List Zp_25519.
+require import Curve25519_Spec.
+require import Curve25519_Hop1.
+require import Curve25519_Hop2.
+require import Curve25519_ref4.
+require import W64limbs.
+from Jasmin require import JWord JWord_array.
+import Zp_25519 Curve25519_Spec Curve25519_Hop2 Curve25519_ref4 Array4 Array32.
+
+type Rep4 = W64.t Array4.t.
+type Rep32 = W8.t Array32.t.
+
+
+op valRep4  (x : Rep4) : int = val_limbs64 (Array4.to_list x).
+op valRep4List  (x : W64.t list) : int = val_limbs64(x).
+op inzpRep4 (x : Rep4) : zp  = inzp (valRep4 x) axiomatized by inzpRep4E.
+op inzpRep4List (x: W64.t list) : zp = inzp (valRep4List x) axiomatized by inzpRep4ListE.
+
+abbrev zpcgrRep4 (x : Rep4) (z : int) : bool = zpcgr (valRep4 x) z.
+
+op valRep32  (x : Rep32) : int = val_limbs8 (Array32.to_list x).
+op inzpRep32 (x : Rep32) : zp  = inzp (valRep32 x) axiomatized by inzpRep32E.
+
+
+(** step 0 : add sub mul sqr - all done by auto **)
+
+equiv eq_h4_add : MHop2.add ~ M.__add4_rrs:
+   f{1} = inzpRep4 f{2} /\
+   g{1} = inzpRep4 g{2}
+    ==>
+   res{1} = inzpRep4 res{2}.
+proof. 
+ proc.  
+ admit.
+qed.
+
+equiv eq_h4_sub : MHop2.sub ~ M.__sub4_rrs:
+   f{1} = inzpRep4 f{2} /\
+   g{1} = inzpRep4 gs{2}
+    ==>
+   res{1} = inzpRep4 res{2}.
+proof.
+proc.
+admit.
+qed.
+
+equiv eq_h4_mul_a24 : MHop2.mul_a24 ~ M.__mul4_a24_rs:
+   f{1} = inzpRep4 xa{2} /\
+   a24{1} = to_uint a24{2}
+    ==>
+   res{1} = inzpRep4 res{2}.
+proof.
+  proc.
+ admit.
+qed.
+
+equiv eq_h4_mul_rss : MHop2.mul ~ M.__mul4_rss:
+   f{1} = inzpRep4 xa{2} /\
+   g{1} = inzpRep4 ya{2}
+    ==>
+   res{1} = inzpRep4 res{2}.
+proof.
+proc.
+admit.
+qed.
+
+equiv eq_h4_sqr : MHop2.sqr ~ M.__sqr4_rs:
+    f{1} = inzpRep4 xa{2}
+    ==>
+    res{1} = inzpRep4 res{2}.
+proof.
+admit.
+qed.
+
+(** step 0.5 : transitivity stuff **)
+equiv eq_h4_add_ssr : MHop2.add ~ M.__add4_ssr:
+   f{1} = inzpRep4 fs{2} /\
+   g{1} = inzpRep4 g{2}
+    ==>
+   res{1} = inzpRep4 res{2}.
+proof.
+proc.
+admit.
+qed.
+
+
+equiv eq_h4_add_sss : MHop2.add ~ M.__add4_sss:
+   f{1} = inzpRep4 fs{2} /\
+   g{1} = inzpRep4 gs{2}
+    ==>
+   res{1} = inzpRep4 res{2}.
+proof.
+proc.
+admit.
+qed.
+
+equiv eq_h4_add_rrs : MHop2.add ~ M.__add4_rrs:
+   f{1} = inzpRep4 f{2} /\
+   g{1} = inzpRep4 g{2}
+    ==>
+   res{1} = inzpRep4 res{2}.
+proof.
+proc.
+admit.
+qed.
+
+
+equiv eq_h4_sub_ssr : MHop2.sub ~ M.__sub4_ssr:
+   f{1} = inzpRep4 fs{2} /\
+   g{1} = inzpRep4 g{2}
+    ==>
+   res{1} = inzpRep4 res{2}.
+proof.
+proc.
+admit.
+qed.
+
+equiv eq_h4_sub_rsr : MHop2.sub ~ M.__sub4_rsr:
+   f{1} = inzpRep4 fs{2} /\
+   g{1} = inzpRep4 g{2}
+    ==>
+   res{1} = inzpRep4 res{2}.
+proof.
+proc.
+admit.
+qed.
+
+equiv eq_h4_sub_sss : MHop2.sub ~ M.__sub4_sss:
+   f{1} = inzpRep4 fs{2} /\
+   g{1} = inzpRep4 gs{2}
+    ==>
+   res{1} = inzpRep4 res{2}.
+proof.
+proc.
+admit.
+qed.
+
+equiv eq_h4_mul_a24_ss : MHop2.mul_a24 ~ M.__mul4_a24_ss:
+   f{1} = inzpRep4 xa{2} /\
+   a24{1} = to_uint a24{2}
+    ==>
+   res{1} = inzpRep4 res{2}.
+proof.
+proc.
+admit.
+qed.
+
+equiv eq_h4_mul_sss : MHop2.mul ~ M.__mul4_sss:
+   f{1} = inzpRep4 xa{2} /\
+   g{1} = inzpRep4 ya{2}
+    ==>
+   res{1} = inzpRep4 res{2}.
+proof.
+proc.
+admit.
+qed.
+
+equiv eq_h4_mul_pp : MHop2.mul ~ M._mul4_pp:
+   f{1} = inzpRep4 xa{2} /\
+   g{1} = inzpRep4 ya{2}
+    ==>
+   res{1} = inzpRep4 res{2}.
+proof.
+proc.
+admit.
+qed.
+
+
+equiv eq_h4_mul_ss : MHop2.mul ~ M._mul4_ss_:
+   f{1} = inzpRep4 xa{2} /\
+   g{1} = inzpRep4 ya{2}
+    ==>
+   res{1} = inzpRep4 res{2}.
+proof.
+proc.
+admit.
+qed.
+
+
+equiv eq_h4_sqr_rs : MHop2.sqr ~ M.__sqr4_rs:
+    f{1} = inzpRep4 xa{2}
+    ==>
+    res{1} = inzpRep4 res{2}.
+proof.
+proc.
+admit.
+qed.
+
+equiv eq_h4_sqr_ss : MHop2.sqr ~ M._sqr4_ss_:
+    f{1} = inzpRep4 xa{2}
+    ==>
+    res{1} = inzpRep4 res{2}.
+proof.
+proc.
+admit.
+qed.
+
+equiv eq_h4_sqr_ss_ : MHop2.sqr ~ M.__sqr4_ss:
+    f{1} = inzpRep4 xa{2}
+    ==>
+    res{1} = inzpRep4 res{2}.
+proof.
+proc.
+admit.
+qed.
+
+equiv eq_h4_sqr_s_ : MHop2.sqr ~ M._sqr4_s_:
+    f{1} = inzpRep4 x{2}
+    ==>
+    res{1} = inzpRep4 res{2}.
+proof.
+proc.
+admit.
+qed.
+
+equiv eq_h4_sqr_p : MHop2.sqr ~ M._sqr4_p:
+    f{1} = inzpRep4 xa{2}
+    ==>
+    res{1} = inzpRep4 res{2}.
+proof.
+proc.
+admit.
+qed.
+
+
+(** step 1 : decode_scalar_25519 **)
+ equiv eq_h4_decode_scalar_25519 :
+  MHop2.decode_scalar ~ M.__decode_scalar:
+  inzp(W256.to_uint(k'{1})) = inzpRep4 k{2}
+  ==> 
+   inzp(W256.to_uint res{1}) = inzpRep32  res{2}. 
+proof.
+admit. (* AUTO *)
+qed.
+
+
+(** step 2 : decode_u_coordinate **)
+equiv eq_h4_decode_u_coordinate :
+  MHop2.decode_u_coordinate ~ M.__decode_u_coordinate4:
+  inzp(W256.to_uint(u'{1})) = inzpRep4 u{2}
+  ==> 
+  res{1} = inzpRep4 res{2}.
+proof.
+admit. (* AUTO MSB already 0 -  ask tiago *)
+qed.
+
+(** step 3 : ith_bit **)
+equiv eq_h4_ith_bit :
+  MHop2.ith_bit ~ M.__ith_bit :
+  inzp (W256.to_uint k'{1}) = inzpRep32 k{2} /\  (ctr{1} = to_uint ctr{2}) ==> b2i res{1} = to_uint res{2}.
+proof.
+proc.
+admit. (* AUTO *)
+qed.
+
+
+(** step 10 : encode point **)
+equiv eq_h4_encode_point : 
+  MHop2.encode_point ~ M.__encode_point4:
+  x2{1} = inzpRep4 x2{2} /\ 
+  z2{1} = inzpRep4 z2r{2}
+  ==>
+  inzp (to_uint res{1}) =  inzpRep4 res{2}.
+proof.
+admit. (* AUTO *)
+qed.
