README.md
@@ -1,15 +1,21 @@
 # X25519-Libjc-EasyCrypt-Proof
 Bringing some libjc X25519 Jasmin-Easycrypt proofs up-to-date (WIP).
 
-Below are files that run without errors as of writing and do not include `admit.` or `smt.`. Note that the imports may need some tinkering around with as my emacs path is broken for whatever reason.
+Below are files that run without errors as of writing and do not include `admit.` or `smt.`. 
 
 - [X] EClib.ec 
-- [X] W64limbs.ec (* warning, contains one lemma that currently results in false but it is probably not be necessary *)
+- [X] W64limbs.ec 
+    - Requires some pruning for unused lemmas that do not prove anything relevant for this scenario.
+    - Contains  one lemma that currently results in false but it is probably not be necessary and can be removed.
 - [X] Zp_25519.ec
+- [X] Curve25519_auto.ec
+    - Everything that is to be proven in Cryptoline, hence all lemmas are admitted for now.
 - [X] Curve25519_spec.ec
 - [X] Curve25519_Hop1.ec
-- [X] Curve25519_Hop2.ec (* includes one lemma that ends in admit as Easycrypt does not like assigning variables to its (i.e h <@ sqr(h)), but the lemma is clearly true *)
+- [ ] Curve25519_Hop2.ec 
+    - Includes two lemmas that end in `admit` because Easycrypt is a bit weird with assigning variables "to themselves" (e.g. `h <@ sqr(h)`) and I am still figuring out how to approach the montgomery ladder proof considering the spec's updated code.
 - [X] Curve25519_Hop3.ec
 - [ ] Curve25519_Hop4.ec
-
+    - All lemmas with names `*_ptr`, `*itr_sqr_s*`, `*jade*` (in total, 6) are admitted as I need to learn about dealing with pointers in Easycrypt. However, the bulk of the work has already been done as their non-pointer versions have been proved. 
+    
 The original Easycrypt files can be found [in the x25519 branch in libjc](https://github.com/tfaoliveira/libjc/tree/x25519/proof/crypto_scalarmult/curve25519).
